Weidenbach_Book/IsaSAT_Sorting_LLVM.thy
@@ -7,56 +7,6 @@ no_notation WB_More_Refinement.fref ("[_]\<^sub>f _ \<rightarrow> _" [0,60,60] 6
 no_notation WB_More_Refinement.freft ("_ \<rightarrow>\<^sub>f _" [60,60] 60)
 declare \<alpha>_butlast[simp del]
 
-definition idx_cdom :: "arena \<Rightarrow> nat set" where
- "idx_cdom arena \<equiv> {i. valid_sort_clause_score_pre_at arena i}"
-
-definition mop_clause_score_less where
-  \<open>mop_clause_score_less arena i j = do {
-    ASSERT(valid_sort_clause_score_pre_at arena i);
-    ASSERT(valid_sort_clause_score_pre_at arena j);
-    RETURN (clause_score_ordering (clause_score_extract arena i) (clause_score_extract arena j))
-  }\<close>
-
-sepref_register clause_score_extract
-
-sepref_def (in -) clause_score_extract_code
-  is \<open>uncurry (RETURN oo clause_score_extract)\<close>
-  :: \<open>[uncurry valid_sort_clause_score_pre_at]\<^sub>a
-      arena_fast_assn\<^sup>k *\<^sub>a sint64_nat_assn\<^sup>k \<rightarrow> uint32_nat_assn *a uint32_nat_assn\<close>
-  supply [[goals_limit = 1]]
-  unfolding clause_score_extract_def valid_sort_clause_score_pre_at_def
-  apply (annot_unat_const "TYPE(32)")
-  by sepref
-
-sepref_def (in -) clause_score_ordering_code
-  is \<open>uncurry (RETURN oo clause_score_ordering)\<close>
-  :: \<open>(uint32_nat_assn *a uint32_nat_assn)\<^sup>k *\<^sub>a (uint32_nat_assn *a uint32_nat_assn)\<^sup>k \<rightarrow>\<^sub>a bool1_assn\<close>
-  supply [[goals_limit = 1]]
-  unfolding clause_score_ordering_def
-  by sepref
-
-sepref_register mop_clause_score_less clause_score_less clause_score_ordering
-sepref_def mop_clause_score_less_impl
-  is \<open>uncurry2 mop_clause_score_less\<close>
-  :: \<open>arena_fast_assn\<^sup>k *\<^sub>a sint64_nat_assn\<^sup>k *\<^sub>a sint64_nat_assn\<^sup>k \<rightarrow>\<^sub>a bool1_assn\<close>
-  unfolding mop_clause_score_less_def
-  by sepref
-
-
-interpretation LBD: weak_ordering_on_lt where
-  C = "idx_cdom vs" and
-  less = "clause_score_less vs"
-  by unfold_locales
-   (auto simp: clause_score_less_def clause_score_extract_def
-      clause_score_ordering_def split: if_splits)
-
-interpretation LBD: parameterized_weak_ordering idx_cdom clause_score_less
-    mop_clause_score_less
-  by unfold_locales
-   (auto simp: mop_clause_score_less_def
-     idx_cdom_def clause_score_less_def)
-
-
 locale pure_eo_adapter =
   fixes elem_assn :: "'a \<Rightarrow> 'ai::llvm_rep \<Rightarrow> assn"
     and wo_assn :: "'a list \<Rightarrow> 'oi::llvm_rep \<Rightarrow> assn"
@@ -176,12 +126,6 @@ begin
       done
 
   end
-  thm mop_eo_extract_def
-
-
-  find_theorems mop_eo_set mop_list_set
-
-  thm mop_eo_set_alt
 
   lemma id_Some_only_some_rel: "(id, Some) \<in> Id \<rightarrow> only_some_rel"
     by (auto simp: only_some_rel_def)
@@ -234,56 +178,7 @@ begin
     wo_set_impl
     by (rule random_access_iterator)
 
-
-  find_theorems "?a = UNPROTECT ?a"
-
 end
-
-
-
-global_interpretation LBD: parameterized_sort_impl_context
-  "woarray_assn snat_assn" "eoarray_assn snat_assn" snat_assn
-  return return
-  eo_extract_impl
-  array_upd
-  idx_cdom clause_score_less mop_clause_score_less mop_clause_score_less_impl
-  "arena_fast_assn"
-  defines
-          LBD_is_guarded_insert_impl = LBD.is_guarded_param_insert_impl
-      and LBD_is_unguarded_insert_impl = LBD.is_unguarded_param_insert_impl
-      and LBD_unguarded_insertion_sort_impl = LBD.unguarded_insertion_sort_param_impl
-      and LBD_guarded_insertion_sort_impl = LBD.guarded_insertion_sort_param_impl
-      and LBD_final_insertion_sort_impl = LBD.final_insertion_sort_param_impl
-      (*and LBD_mop_lchild_impl  = LBD.mop_lchild_impl
-      and LBD_mop_rchild_impl  = LBD.mop_rchild_impl
-      and LBD_has_rchild_impl  = LBD.has_rchild_impl
-      and LBD_has_lchild_impl  = LBD.has_lchild_impl *)
-
-      and LBD_pcmpo_idxs_impl  = LBD.pcmpo_idxs_impl
-      and LBD_pcmpo_v_idx_impl  = LBD.pcmpo_v_idx_impl
-      and LBD_pcmpo_idx_v_impl  = LBD.pcmpo_idx_v_impl
-      and LBD_pcmp_idxs_impl  = LBD.pcmp_idxs_impl
-
-      and LBD_mop_geth_impl    = LBD.mop_geth_impl
-      and LBD_mop_seth_impl    = LBD.mop_seth_impl
-      and LBD_sift_down_impl   = LBD.sift_down_impl
-      and LBD_heapify_btu_impl = LBD.heapify_btu_impl
-      and LBD_heapsort_impl    = LBD.heapsort_param_impl
-      and LBD_qsp_next_l_impl       = LBD.qsp_next_l_impl
-      and LBD_qsp_next_h_impl       = LBD.qsp_next_h_impl
-      and LBD_qs_partition_impl     = LBD.qs_partition_impl
-(*      and LBD_qs_partitionXXX_impl     = LBD.qs_partitionXXX_impl *)
-      and LBD_partition_pivot_impl  = LBD.partition_pivot_impl
-      and LBD_introsort_aux_impl = LBD.introsort_aux_param_impl
-      and LBD_introsort_impl        = LBD.introsort_param_impl
-      and LBD_move_median_to_first_impl = LBD.move_median_to_first_param_impl
-
-  apply unfold_locales
-  apply (rule eo_hnr_dep)+
-  unfolding GEN_ALGO_def refines_param_relp_def (* TODO: thm gen_refines_param_relpI *)
-  by (rule mop_clause_score_less_impl.refine)
-
-
 
 lemma al_pure_eo: "is_pure A \<Longrightarrow> pure_eo_adapter A (al_assn A) arl_nth arl_upd"
   apply unfold_locales
@@ -306,66 +201,6 @@ lemma al_pure_eo: "is_pure A \<Longrightarrow> pure_eo_adapter A (al_assn A) arl
       by vcg
     done
   done
-
-
-global_interpretation
-  LBD_it: pure_eo_adapter sint64_nat_assn vdom_fast_assn arl_nth arl_upd
-  defines LBD_it_eo_extract_impl = LBD_it.eo_extract_impl
-  apply (rule al_pure_eo)
-  by simp
-
-
-
-global_interpretation LBD_it: parameterized_sort_impl_context
-  vdom_fast_assn "LBD_it.eo_assn" sint64_nat_assn
-  return return
-  LBD_it_eo_extract_impl
-  arl_upd
-  idx_cdom clause_score_less mop_clause_score_less mop_clause_score_less_impl
-  "arena_fast_assn"
-  defines
-          LBD_it_is_guarded_insert_impl = LBD_it.is_guarded_param_insert_impl
-      and LBD_it_is_unguarded_insert_impl = LBD_it.is_unguarded_param_insert_impl
-      and LBD_it_unguarded_insertion_sort_impl = LBD_it.unguarded_insertion_sort_param_impl
-      and LBD_it_guarded_insertion_sort_impl = LBD_it.guarded_insertion_sort_param_impl
-      and LBD_it_final_insertion_sort_impl = LBD_it.final_insertion_sort_param_impl
-      (*and LBD_it_mop_lchild_impl  = LBD_it.mop_lchild_impl
-      and LBD_it_mop_rchild_impl  = LBD_it.mop_rchild_impl
-      and LBD_it_has_rchild_impl  = LBD_it.has_rchild_impl
-      and LBD_it_has_lchild_impl  = LBD_it.has_lchild_impl *)
-
-      and LBD_it_pcmpo_idxs_impl  = LBD_it.pcmpo_idxs_impl
-      and LBD_it_pcmpo_v_idx_impl  = LBD_it.pcmpo_v_idx_impl
-      and LBD_it_pcmpo_idx_v_impl  = LBD_it.pcmpo_idx_v_impl
-      and LBD_it_pcmp_idxs_impl  = LBD_it.pcmp_idxs_impl
-
-      and LBD_it_mop_geth_impl    = LBD_it.mop_geth_impl
-      and LBD_it_mop_seth_impl    = LBD_it.mop_seth_impl
-      and LBD_it_sift_down_impl   = LBD_it.sift_down_impl
-      and LBD_it_heapify_btu_impl = LBD_it.heapify_btu_impl
-      and LBD_it_heapsort_impl    = LBD_it.heapsort_param_impl
-      and LBD_it_qsp_next_l_impl       = LBD_it.qsp_next_l_impl
-      and LBD_it_qsp_next_h_impl       = LBD_it.qsp_next_h_impl
-      and LBD_it_qs_partition_impl     = LBD_it.qs_partition_impl
-(*      and LBD_it_qs_partitionXXX_impl     = LBD_it.qs_partitionXXX_impl *)
-      and LBD_it_partition_pivot_impl  = LBD_it.partition_pivot_impl
-      and LBD_it_introsort_aux_impl = LBD_it.introsort_aux_param_impl
-      and LBD_it_introsort_impl        = LBD_it.introsort_param_impl
-      and LBD_it_move_median_to_first_impl = LBD_it.move_median_to_first_param_impl
-
-  apply unfold_locales
-  unfolding GEN_ALGO_def refines_param_relp_def (* TODO: thm gen_refines_param_relpI *)
-  apply (rule mop_clause_score_less_impl.refine)
-  done
-
-
-
-lemmas [llvm_inline] = LBD_it.eo_extract_impl_def[THEN meta_fun_cong, THEN meta_fun_cong]
-
-print_named_simpset llvm_inline
-export_llvm
-  "LBD_heapsort_impl :: _ \<Rightarrow> _ \<Rightarrow> _"
-  "LBD_introsort_impl :: _ \<Rightarrow> _ \<Rightarrow> _"
 
 
 end
